obfuscate_age

src/tls/Negotiation.Writers.Aux.fst
@@ -1,9 +1,26 @@
 module Negotiation.Writers.Aux
 
 friend Parsers.PskBinderEntry
+friend Parsers.PskIdentity
 
+module LWP = LowParseWriters.Compat
 module LP = LowParse.Spec
 
 let valid_pskBinderEntry_intro =
    [@inline_let] let _ = assert_norm (Parsers.PskBinderEntry.pskBinderEntry == LowParse.Spec.Bytes.parse_bounded_vlbytes_t 32 255) in
    LWP.valid_synth_parser_eq (LWP.parse_vlbytes 32ul 255ul) Parsers.PskBinderEntry.lwp_pskBinderEntry
+
+let valid_pskIdentity_intro =
+  let open Parsers.PskIdentity in
+  assert_norm (pskIdentity' == LP.get_parser_type pskIdentity'_parser);
+  assert_norm (pskIdentity_parser_kind == pskIdentity'_parser_kind);
+  synth_pskIdentity_injective ();
+  synth_pskIdentity_inverse ();
+  LWP.valid_synth_implies _ _ _ _
+  (LWP.valid_synth_compose
+    _ _ _ _
+    (LWP.valid_synth_parse_synth (lwp_pskIdentity_identity `LWP.star` LWP.parse_u32) synth_pskIdentity synth_pskIdentity_recip ())
+    _ _ _
+    (LWP.valid_synth_parser_eq (LWP.parse_synth (lwp_pskIdentity_identity `LWP.star` LWP.parse_u32) synth_pskIdentity synth_pskIdentity_recip) lwp_pskIdentity)
+  )
+  _ _
