src/tls/Negotiation.Writers.fst
@@ -26,6 +26,7 @@ open Negotiation
 let write_binder_ph'
   (#inv: LWP.memory_invariant)
   (tc: LWP.ptr Parsers.TicketContents13.lwp_ticketContents13 inv)
+  ()
 : LWP.Write unit LWP.emp lwp_pskBinderEntry (fun _ -> True) (fun _ _ out -> out == compute_binder_ph_new (LWP.deref_spec tc)) inv
 =
   let c = LWP.deref CipherSuite.cipherSuite13_reader (LWP.access Parsers.TicketContents13.lwp_ticketContents13 Parsers.CipherSuite13.lwp_cipherSuite13 Parsers.TicketContents13.accessor_ticketContents13_cs tc) in
@@ -84,6 +85,30 @@ let write_binder_ph
     B.fill (B.sub sout.LP.base pout_payload len) 0uy len;
     pskBinderEntry_finalize sout pout_from len
   end
+
+#pop-options
+
+#restart-solver
+
+let write_obfuscate_age'
+  (#inv: LWP.memory_invariant)
+  (now: U32.t)
+  (ri: LWP.ptr Parsers.ResumeInfo13.lwp_resumeInfo13 inv)
+  ()
+: LWP.Write unit LWP.emp Parsers.PskIdentity.lwp_pskIdentity (fun _ -> True) (fun _ _ out -> out == obfuscate_age_new now (LWP.deref_spec ri)) inv
+=
+  LWP.cat (LWP.access Parsers.ResumeInfo13.lwp_resumeInfo13 Parsers.PskIdentity.lwp_pskIdentity_identity Parsers.ResumeInfo13.accessor_resumeInfo13_identity ri);
+  let tk = LWP.access Parsers.ResumeInfo13.lwp_resumeInfo13 Parsers.TicketContents13.lwp_ticketContents13 Parsers.ResumeInfo13.accessor_resumeInfo13_ticket ri in
+  let creation_time = LWP.deref LowParse.Low.Int.read_u32 (LWP.access Parsers.TicketContents13.lwp_ticketContents13 LWP.parse_u32 Parsers.TicketContents13.accessor_ticketContents13_creation_time tk) in
+  let age = FStar.UInt32.((now -%^ creation_time) *%^ 1000ul) in
+  let age_add = LWP.deref LowParse.Low.Int.read_u32 (LWP.access Parsers.TicketContents13.lwp_ticketContents13 LWP.parse_u32 Parsers.TicketContents13.accessor_ticketContents13_age_add tk) in
+  let obfuscated_age = PSK.encode_age age age_add in
+  LWP.append LWP.parse_u32 LowParse.Low.Int.write_u32 obfuscated_age;
+  LWP.valid_synth _ _ _ _ _ Aux.valid_pskIdentity_intro
+
+#push-options "--z3rlimit 64 --query_stats"
+
+#restart-solver
 
 let write_obfuscate_age
   (now: U32.t)
